Cleaned up Assertion and Hoare syntax and implementation some more.

SoftwareFoundations/ProgrammingLanguageFoundations/Hoare.lean
@@ -13,7 +13,53 @@ namespace SoftwareFoundations.ProgrammingLanguageFoundations.Hoare
   -/
 
   def Assertion: Type := State → Prop
+
+  @[reducible] def Assertion.prop (P: Prop): Assertion
+    | _ => P
+  @[reducible] def Assertion.implies (P Q: Assertion): Assertion
+    | s => P s → Q s
+  @[reducible] def Assertion.iff (P Q: Assertion): Assertion
+    | s => P s ↔ Q s
+  @[reducible] def Assertion.and (P Q: Assertion): Assertion
+    | s => P s ∧ Q s
+  @[reducible] def Assertion.or (P Q: Assertion): Assertion
+    | s => P s ∨ Q s
+  @[reducible] def Assertion.not (P: Assertion): Assertion
+    | s => ¬ P s
+
   def NatAssertion: Type := State → Nat
+
+  @[reducible] def NatAssertion.num (n: Nat): NatAssertion
+    | _ => n
+  @[reducible] def NatAssertion.id (id: String): NatAssertion
+    | s => s id
+  @[reducible] def NatAssertion.arith (e: Arith): NatAssertion
+    | s => e.eval s
+
+  @[reducible] def NatAssertion.plus (e₁ e₂: NatAssertion): NatAssertion
+    | s => e₁ s + e₂ s
+  @[reducible] def NatAssertion.minus (e₁ e₂: NatAssertion): NatAssertion
+    | s => e₁ s - e₂ s
+  @[reducible] def NatAssertion.mult (e₁ e₂: NatAssertion): NatAssertion
+    | s => e₁ s * e₂ s
+
+  @[reducible] def NatAssertion.app₁ (f: Nat → Nat) (e: NatAssertion): NatAssertion
+    | s => f (e s)
+  @[reducible] def NatAssertion.app₂ (f: Nat → Nat → Nat) (e₁ e₂: NatAssertion): NatAssertion
+    | s => f (e₁ s) (e₂ s)
+
+  @[reducible] def NatAssertion.eq (P Q: NatAssertion): Assertion
+    | s => P s = Q s
+  @[reducible] def NatAssertion.neq (P Q: NatAssertion): Assertion
+    | s => P s ≠ Q s
+  @[reducible] def NatAssertion.le (P Q: NatAssertion): Assertion
+    | s => P s ≤ Q s
+  @[reducible] def NatAssertion.lt (P Q: NatAssertion): Assertion
+    | s => P s < Q s
+  @[reducible] def NatAssertion.ge (P Q: NatAssertion): Assertion
+    | s => P s ≥ Q s
+  @[reducible] def NatAssertion.gt (P Q: NatAssertion): Assertion
+    | s => P s > Q s
 
   section
     private def assertionOne: Assertion
@@ -35,19 +81,25 @@ namespace SoftwareFoundations.ProgrammingLanguageFoundations.Hoare
   syntax:70 nat_assert:70 "*" nat_assert:71 : nat_assert
   syntax:30 "app₁" "‹" term "›" nat_assert : nat_assert
   syntax:30 "app₂" "‹" term "›" nat_assert nat_assert : nat_assert
+  syntax "‹num:" term "›" : nat_assert
+  syntax "‹id:" term "›" : nat_assert
+  syntax "‹arith:" arith "›" : nat_assert
   syntax "(" nat_assert ")" : nat_assert
 
   syntax "[NatAssert|" nat_assert "]" : term
 
   macro_rules
-    | `([NatAssert| $n:num])                                     => `(((fun _ => $n): NatAssertion))
-    | `([NatAssert| $id:ident])                                  => `(((fun s => s $(Lean.quote (toString id.getId))): NatAssertion))
-    | `([NatAssert| $x + $y])                                    => `(((fun s => ([NatAssert| $x] s) + ([NatAssert| $y] s)): NatAssertion))
-    | `([NatAssert| $x - $y])                                    => `(((fun s => ([NatAssert| $x] s) - ([NatAssert| $y] s)): NatAssertion))
-    | `([NatAssert| $x * $y])                                    => `(((fun s => ([NatAssert| $x] s) * ([NatAssert| $y] s)): NatAssertion))
-    | `([NatAssert| app₂ ‹$f:term› $x:nat_assert $y:nat_assert]) => `(((fun s => $(Lean.quote f) ([NatAssert| $x] s) ([NatAssert| $y] s)): NatAssertion))
-    | `([NatAssert| app₁ ‹$f:term› $x:nat_assert])               => `(((fun s => $(Lean.quote f) ([NatAssert| $x] s)): NatAssertion))
-    | `([NatAssert| ( $a:nat_assert )])                          => `([NatAssert| $a])
+    | `([NatAssert| $n:num])                                       => `(NatAssertion.num $n)
+    | `([NatAssert| ‹num: $n:term ›])                              => `(NatAssertion.num $(Lean.quote n))
+    | `([NatAssert| $id:ident])                                    => `(NatAssertion.id $(Lean.quote (toString id.getId)))
+    | `([NatAssert| ‹id: $id:term ›])                              => `(NatAssertion.id $(Lean.quote id))
+    | `([NatAssert| ‹arith: $e:arith ›])                           => `(NatAssertion.arith [Arith| $e])
+    | `([NatAssert| $x + $y])                                      => `(NatAssertion.plus [NatAssert| $x] [NatAssert| $y])
+    | `([NatAssert| $x - $y])                                      => `(NatAssertion.minus [NatAssert| $x] [NatAssert| $y])
+    | `([NatAssert| $x * $y])                                      => `(NatAssertion.mult [NatAssert| $x] [NatAssert| $y])
+    | `([NatAssert| app₂ ‹ $f:term › $x:nat_assert $y:nat_assert]) => `(NatAssertion.app₂ $(Lean.quote f) [NatAssert| $x] [NatAssert| $y])
+    | `([NatAssert| app₁ ‹ $f:term › $x:nat_assert])               => `(NatAssertion.app₁ $(Lean.quote f) [NatAssert| $x])
+    | `([NatAssert| ( $a:nat_assert )])                            => `([NatAssert| $a])
 
   section
     example: [NatAssert| 42] [State|] = 42 := rfl
@@ -89,19 +141,19 @@ namespace SoftwareFoundations.ProgrammingLanguageFoundations.Hoare
   syntax "[Assert|" assert "]" : term
 
   macro_rules
-    | `([Assert| ‹prop: $P:term › ])             => `(((fun _ => $(Lean.quote P)): Assertion))
-    | `([Assert| ‹$P:term› ])                    => `($(Lean.quote P))
-    | `([Assert| $P → $Q])                       => `(((fun s => [Assert| $P] s → [Assert| $Q] s): Assertion))
-    | `([Assert| $P ↔ $Q])                       => `(((fun s => [Assert| $P] s ↔ [Assert| $Q] s): Assertion))
-    | `([Assert| $P ∧ $Q])                       => `(((fun s => [Assert| $P] s ∧ [Assert| $Q] s): Assertion))
-    | `([Assert| $P ∨ $Q])                       => `(((fun s => [Assert| $P] s ∨ [Assert| $Q] s): Assertion))
-    | `([Assert| ¬ $P])                          => `(((fun s => ¬ [Assert| $P] s): Assertion))
-    | `([Assert| $P:nat_assert = $Q:nat_assert]) => `(((fun s => [NatAssert| $P] s = [NatAssert| $Q] s): Assertion))
-    | `([Assert| $P:nat_assert ≠ $Q:nat_assert]) => `(((fun s => [NatAssert| $P] s ≠ [NatAssert| $Q] s): Assertion))
-    | `([Assert| $P:nat_assert ≤ $Q:nat_assert]) => `(((fun s => [NatAssert| $P] s ≤ [NatAssert| $Q] s): Assertion))
-    | `([Assert| $P:nat_assert < $Q:nat_assert]) => `(((fun s => [NatAssert| $P] s < [NatAssert| $Q] s): Assertion))
-    | `([Assert| $P:nat_assert ≥ $Q:nat_assert]) => `(((fun s => [NatAssert| $P] s ≥ [NatAssert| $Q] s): Assertion))
-    | `([Assert| $P:nat_assert > $Q:nat_assert]) => `(((fun s => [NatAssert| $P] s > [NatAssert| $Q] s): Assertion))
+    | `([Assert| ‹prop: $P:term › ])             => `(Assertion.prop $(Lean.quote P))
+    | `([Assert| ‹ $P:term › ])                  => `($(Lean.quote P))
+    | `([Assert| $P → $Q])                       => `(Assertion.implies [Assert| $P] [Assert| $Q])
+    | `([Assert| $P ↔ $Q])                       => `(Assertion.iff     [Assert| $P] [Assert| $Q])
+    | `([Assert| $P ∧ $Q])                       => `(Assertion.and     [Assert| $P] [Assert| $Q])
+    | `([Assert| $P ∨ $Q])                       => `(Assertion.or      [Assert| $P] [Assert| $Q])
+    | `([Assert| ¬ $P])                          => `(Assertion.not     [Assert| $P])
+    | `([Assert| $P:nat_assert = $Q:nat_assert]) => `(NatAssertion.eq  [NatAssert| $P] [NatAssert| $Q])
+    | `([Assert| $P:nat_assert ≠ $Q:nat_assert]) => `(NatAssertion.neq [NatAssert| $P] [NatAssert| $Q])
+    | `([Assert| $P:nat_assert ≤ $Q:nat_assert]) => `(NatAssertion.le  [NatAssert| $P] [NatAssert| $Q])
+    | `([Assert| $P:nat_assert < $Q:nat_assert]) => `(NatAssertion.lt  [NatAssert| $P] [NatAssert| $Q])
+    | `([Assert| $P:nat_assert ≥ $Q:nat_assert]) => `(NatAssertion.ge  [NatAssert| $P] [NatAssert| $Q])
+    | `([Assert| $P:nat_assert > $Q:nat_assert]) => `(NatAssertion.gt  [NatAssert| $P] [NatAssert| $Q])
     | `([Assert| ( $a:assert )])                 => `([Assert| $a])
 
   section
@@ -133,7 +185,22 @@ namespace SoftwareFoundations.ProgrammingLanguageFoundations.Hoare
 
   @[reducible]
   def HoareTriple (P: Assertion) (c: Command) (Q: Assertion): Prop :=
-    ∀ s₁ s₂: State, P s₁ → CommandEval c s₁ s₂ → Q s₂
+    ∀ s₁ s₂: State, P s₁ → (s₁ =[c]=> s₂) → Q s₂
+
+  @[reducible]
+  def Assertion.subst (id: String) (e: Arith) (P: Assertion): Assertion
+    | s => P (s.update id (e.eval s))
+
+  syntax:40 assert "[" ident "↦" arith "]" : assert
+  syntax:40 assert "[" "‹" term "›" "↦" arith "]" : assert
+  syntax:40 assert "[" ident "↦" "‹" term "›" "]" : assert
+  syntax:40 assert "[" "‹" term "›" "↦" "‹" term "›" "]" : assert
+
+  macro_rules
+    | `([Assert| $P:assert [ $id:ident ↦ $e:arith ]])       => `([Assert| $P].subst $(Lean.quote (toString id.getId)) [Arith| $e])
+    | `([Assert| $P:assert [ $id:ident ↦ ‹ $e:term › ]])    => `([Assert| $P].subst $(Lean.quote (toString id.getId)) $(Lean.quote e))
+    | `([Assert| $P:assert [ ‹ $id:term › ↦ $e:arith ]])    => `([Assert| $P].subst $(Lean.quote id) [Arith| $e])
+    | `([Assert| $P:assert [ ‹ $id:term › ↦ ‹ $e:term › ]]) => `([Assert| $P].subst $(Lean.quote id) $(Lean.quote e))
 
   declare_syntax_cat hoare
 
@@ -145,11 +212,10 @@ namespace SoftwareFoundations.ProgrammingLanguageFoundations.Hoare
     | `([Hoare| ⦃ $pre:assert ⦄ $c:cmd ⦃ $post:assert ⦄ ]) => `(HoareTriple [Assert| $pre] [Imp| $c] [Assert| $post])
 
   theorem HoareTriple.post_true {P Q: Assertion} {c: Command}: (h: (s: State) → Q s) → [Hoare| ⦃ ‹P› ⦄ ‹c› ⦃ ‹Q› ⦄]
-    | h, s₁, s₂, hp, c =>
-      [Hoare| ⦃ ‹prop:h s₁› ⦄ ‹c› ⦃ ‹hp› ⦄]
+    | h, _, _, _, _ => h _
 
   theorem HoareTriple.pre_false {P Q: Assertion} {c: Command}: (h: (s: State) → ¬P s) → [Hoare| ⦃ ‹P› ⦄ ‹c› ⦃ ‹Q› ⦄]
-    | h, s₁, s₂, hp, c => sorry
+    | h, _, _, hp, _ => absurd hp (h _)
 
   /-
   ## Proof Rules
@@ -159,14 +225,14 @@ namespace SoftwareFoundations.ProgrammingLanguageFoundations.Hoare
   ### Skip
   -/
 
-  def HoareTriple.skip {P: Assertion}: [Hoare| ⦃ ‹P› ⦄ skip ⦃ ‹P› ⦄]
+  theorem  HoareTriple.skip {P: Assertion}: [Hoare| ⦃ ‹P› ⦄ skip ⦃ ‹P› ⦄]
     | _, _, hp, .skip _ => hp
 
   /-
   ### Sequencing
   -/
 
-  def HoareTriple.seq {P Q R: Assertion} {c₁ c₂: Command} (h₁: [Hoare| ⦃ ‹Q› ⦄ ‹c₂› ⦃ ‹R› ⦄]) (h₂: [Hoare| ⦃ ‹P› ⦄ ‹c₁› ⦃ ‹Q› ⦄]): [Hoare| ⦃ ‹P› ⦄ ‹c₁›; ‹c₂› ⦃ ‹R› ⦄]
+  theorem HoareTriple.seq {P Q R: Assertion} {c₁ c₂: Command} (h₁: [Hoare| ⦃ ‹Q› ⦄ ‹c₂› ⦃ ‹R› ⦄]) (h₂: [Hoare| ⦃ ‹P› ⦄ ‹c₁› ⦃ ‹Q› ⦄]): [Hoare| ⦃ ‹P› ⦄ ‹c₁›; ‹c₂› ⦃ ‹R› ⦄]
     | _, _, hp, .seq _ _ _ h₃ h₄ =>
       have hq := h₂ _ _ hp h₃
       h₁ _ _ hq h₄
@@ -175,34 +241,56 @@ namespace SoftwareFoundations.ProgrammingLanguageFoundations.Hoare
   ### Assignment
   -/
 
-  @[reducible]
-  def Assertion.subst (id: String) (e: Arith) (P: Assertion): Assertion
-    | s => P (s.update id (e.eval s))
-
-  notation P "[" id "↦" e "]" => Assertion.subst id e P
-
-  def HoareTriple.assign {Q: Assertion} {id: String} {e: Arith}: [Hoare| ⦃Q [id ↦ e]⦄ ‹id› := ‹e›) ⦃Q⦄]
-    | _,_, hqs, .assign _ h =>
+  theorem HoareTriple.assign {Q: Assertion} {id: String} {e: Arith}: [Hoare| ⦃ ‹Q› [‹id› ↦ ‹e›]⦄ ‹id› := ‹e› ⦃ ‹Q› ⦄]
+    | _, _, hq, .assign _ h =>
       have h :=
         calc Assertion.subst id e Q _
           _ = Q (LogicalFoundations.Maps.TotalMap.update _ id (Arith.eval _ e)) := rfl
           _ = Q (LogicalFoundations.Maps.TotalMap.update _ id _)                := congrArg Q (congrArg (LogicalFoundations.Maps.TotalMap.update _ id) h)
       -- TODO: Remove Tactic Block
-      by rw [h] at hqs; exact hqs
+      by rw [h] at hq; exact hq
 
   namespace Term
-    example: [Hoare| ⦃(X < 5) [X ↦ X + 1]⦄ X := X + 1 ⦃X < 5⦄] :=
-      HoareTriple.assign
+    example: [Hoare| ⦃(X < 5) [X ↦ X + 1]⦄ X := X + 1 ⦃X < 5⦄]
+      | s₁, s₂, hq, hc =>
+        by
+          unfold Assertion.subst at hq
+          unfold Arith.eval at hq
+          unfold Arith.eval at hq
+          unfold NatAssertion.lt at hq
+          unfold NatAssertion.num at hq
+          unfold NatAssertion.id at hq
+          unfold NatAssertion.lt
+          unfold NatAssertion.num
+          unfold NatAssertion.id
+          simp_all
 
-    example: ∃ P, [Hoare| ⦃ ‹P› ⦄ X := 2 * X ⦃X ≤ 10⦄] :=
-      ⟨[Assert| X ≤ 5], sorry⟩
+          sorry
 
-    example: ∃ P, [Hoare| ⦃ ‹P› ⦄ X := 3 ⦃(X ≤ 0 ∧ X ≤ 5)⦄] :=
-      ⟨[Assert| ‹prop:True› ], sorry⟩
+    example: ∃ P: Assertion, [Hoare| ⦃ ‹P› ⦄ X := 2 * X ⦃X ≤ 10⦄] :=
+      have w := [Assert| X ≤ 5]
+      have hw
+      | _, _, hq, hc => sorry
+      ⟨w, hw⟩
 
-    example: ∃ E: Arith, ¬ [Hoare| ⦃ ‹prop: True› ⦄ X := ‹e› ⦃X = e⦄] := sorry
-    example (n: Nat) (e: Arith) (P: Assertion): [Hoare| ⦃ ‹fun s => P s ∧ s "X" = n› ⦄ X := ‹e› ⦃ ‹fun s => P (s.update "X" n) ∧ s "X" = e.eval (s.update "X" n)› ⦄] := sorry
-    example (e: Arith) (P: Assertion): [Hoare| ⦃ ‹fun s => P s› ⦄ X := ‹e› ⦃ ‹fun s => ∃ n: Nat, P (s.update "X" n) ∧ s "X" = e.eval (s.update "X" n)› ⦄] := sorry
+    example: ∃ P: Assertion, [Hoare| ⦃ ‹P› ⦄ X := 3 ⦃(X ≤ 0 ∧ X ≤ 5)⦄] :=
+      have w := [Assert| ‹prop:True› ]
+      have hw
+      | _, _, hq, hc => sorry
+      ⟨w, hw⟩
+
+    example: ∃ E: Arith, ¬ [Hoare| ⦃ ‹prop: True› ⦄ X := ‹e› ⦃X = ‹arith:e›⦄] :=
+      have w := sorry
+      have hw := sorry
+      ⟨w, hw⟩
+
+    example (n: Nat) (e: Arith) (P: Assertion): [Hoare| ⦃ ‹P› ∧ X = ‹num:n› ⦄ X := ‹e› ⦃ ‹fun s => P.subst "X" e (s.update "X" n) ∧ s "X" = e.eval (s.update "X" n)› ⦄]
+      | _, _, hq, hc =>
+        sorry
+
+    example (e: Arith) (P: Assertion): [Hoare| ⦃ ‹P› ⦄ X := ‹e› ⦃ ‹fun s => ∃ n: Nat, P (s.update "X" n) ∧ s "X" = e.eval (s.update "X" n)› ⦄]
+      | _, _, hq, hc =>
+        sorry
   end Term
 
   namespace Tactic
@@ -242,7 +330,11 @@ namespace SoftwareFoundations.ProgrammingLanguageFoundations.Hoare
   ### Consequence
   -/
 
-
+  theorem HoareTriple.consequence {P₁ P₂ Q₁ Q₂: Assertion} {c: Command} (h₁: [Hoare| ⦃ ‹P₂› ⦄ ‹c› ⦃ ‹Q₂› ⦄]) (h₂: [Assert| ‹P₁› → ‹P₂›]) (h₃: [Assert| ‹Q₂› → ‹Q₁›]): [Hoare| ⦃ ‹P₁› ⦄ ‹c› ⦃ ‹Q₁› ⦄] :=
+    sorry
+    where
+      pre {P₁ P₂ Q: Assertion} {c: Command} (h₁: [Hoare| ⦃ ‹P₂› ⦄ ‹c› ⦃ ‹Q› ⦄]) (h₂: [Assert| ‹P₁› → ‹P₂›]): [Hoare| ⦃ ‹P₁› ⦄ ‹c› ⦃ ‹Q› ⦄] := sorry
+      post {P Q₁ Q₂: Assertion} {c: Command} (h₁: [Hoare| ⦃ ‹P› ⦄ ‹c› ⦃ ‹Q₂› ⦄]) (h₂: [Assert| ‹Q₂› → ‹Q₁›]): [Hoare| ⦃ ‹P› ⦄ ‹c› ⦃ ‹Q₁› ⦄] := sorry
 
   /-
   ### Automation
